@prefix : <https://w3id.org/fedecom/battery#> .
@prefix owl: <http://www.w3.org/2002/07/owl#> .
@prefix rdf: <http://www.w3.org/1999/02/22-rdf-syntax-ns#> .
@prefix xml: <http://www.w3.org/XML/1998/namespace> .
@prefix xsd: <http://www.w3.org/2001/XMLSchema#> .
@prefix rdfs: <http://www.w3.org/2000/01/rdf-schema#> .
@base <https://w3id.org/fedecom/battery> .

<https://w3id.org/fedecom/battery> rdf:type owl:Ontology ;
                                    owl:imports <https://w3id.org/fedecom/units> ;
                                    <http://creativecommons.org/ns#license> "http://purl.org/NET/rdflicense/cc-by4.0" ;
                                    <http://purl.org/dc/terms/contributor> """Ignacio Lázaro (Tekniker) <ignacio.lazaro@tekniker.es>
Andoni Osorio (Tekniker) <andoni.osorio@tekniker.es>
Marko Jelić (Institut Mihajlo Pupin) <marko.jelic@pupin.rs>
Spyros Tzavikas (Grid Singularity) <spyros@gridsingularity.com>""" ;
                                    <http://purl.org/dc/terms/created> "" ;
                                    <http://purl.org/dc/terms/creator> "Cristina Aceta (Tekniker) <cristina.aceta@tekniker.es>" ;
                                    <http://purl.org/dc/terms/description> "This ontology module includes the necessary classes and properties to model and characterize batteries." ;
                                    <http://purl.org/dc/terms/title> "Battery: Battery Characterization module for the FEDECOM Ontology" ;
                                    <http://purl.org/vocab/vann/preferredNamespacePrefix> "battery" ;
                                    <http://purl.org/vocab/vann/preferredNamespaceUri> "https://w3id.org/fedecom/battery#" ;
                                    owl:versionInfo "" .

#################################################################
#    Annotation properties
#################################################################

###  http://creativecommons.org/ns#license
<http://creativecommons.org/ns#license> rdf:type owl:AnnotationProperty .


###  http://purl.org/dc/terms/contributor
<http://purl.org/dc/terms/contributor> rdf:type owl:AnnotationProperty .


###  http://purl.org/dc/terms/created
<http://purl.org/dc/terms/created> rdf:type owl:AnnotationProperty .


###  http://purl.org/dc/terms/creator
<http://purl.org/dc/terms/creator> rdf:type owl:AnnotationProperty .


###  http://purl.org/dc/terms/description
<http://purl.org/dc/terms/description> rdf:type owl:AnnotationProperty .


###  http://purl.org/dc/terms/title
<http://purl.org/dc/terms/title> rdf:type owl:AnnotationProperty .


###  http://purl.org/vocab/vann/preferredNamespacePrefix
<http://purl.org/vocab/vann/preferredNamespacePrefix> rdf:type owl:AnnotationProperty .


###  http://purl.org/vocab/vann/preferredNamespaceUri
<http://purl.org/vocab/vann/preferredNamespaceUri> rdf:type owl:AnnotationProperty .


###  http://www.w3.org/2002/07/owl#versionInfo
owl:versionInfo rdf:type owl:AnnotationProperty .


###  http://www.w3.org/2003/06/sw-vocab-status/ns#term_status
<http://www.w3.org/2003/06/sw-vocab-status/ns#term_status> rdf:type owl:AnnotationProperty .


###  http://www.w3.org/2004/02/skos/core#example
<http://www.w3.org/2004/02/skos/core#example> rdf:type owl:AnnotationProperty .


#################################################################
#    Object Properties
#################################################################

###  https://w3id.org/fedecom/battery#hasCharacteristic
:hasCharacteristic rdf:type owl:ObjectProperty ;
                   rdfs:comment "Links a battery to a general feature or property that describes its nature, such as chemistry type, capacity, or performance attributes." ;
                   rdfs:label "has characteristic" ;
                   <http://www.w3.org/2003/06/sw-vocab-status/ns#term_status> "stable" .


###  https://w3id.org/fedecom/battery#hasChargeCurrent
:hasChargeCurrent rdf:type owl:ObjectProperty ;
                  rdfs:subPropertyOf :hasCharacteristic ;
                  rdfs:domain :Battery ;
                  rdfs:range :ChargeCurrent ;
                  rdfs:comment "Relates a battery to the value of electric current supplied during charging." ;
                  rdfs:label "has charge current" ;
                  <http://www.w3.org/2003/06/sw-vocab-status/ns#term_status> "stable" .


###  https://w3id.org/fedecom/battery#hasChargePower
:hasChargePower rdf:type owl:ObjectProperty ;
                rdfs:subPropertyOf :hasCharacteristic ;
                rdfs:domain :Battery ;
                rdfs:range :ChargePower ;
                rdfs:comment "Relates a battery to the amount of power delivered during charging." ;
                rdfs:label "has charge power" ;
                <http://www.w3.org/2003/06/sw-vocab-status/ns#term_status> "stable" .


###  https://w3id.org/fedecom/battery#hasDischargeCurrent
:hasDischargeCurrent rdf:type owl:ObjectProperty ;
                     rdfs:subPropertyOf :hasCharacteristic ;
                     rdfs:domain :Battery ;
                     rdfs:range :DischargeCurrent ;
                     rdfs:comment "Relates a battery to the value of electric current drawn during discharge." ;
                     rdfs:label "has discharge current" ;
                     <http://www.w3.org/2003/06/sw-vocab-status/ns#term_status> "stable" .


###  https://w3id.org/fedecom/battery#hasDischargePower
:hasDischargePower rdf:type owl:ObjectProperty ;
                   rdfs:subPropertyOf :hasCharacteristic ;
                   rdfs:domain :Battery ;
                   rdfs:range :DischargePower ;
                   rdfs:comment "Relates a battery to the amount of power output during discharge." ;
                   rdfs:label "has discharge power" ;
                   <http://www.w3.org/2003/06/sw-vocab-status/ns#term_status> "stable" .


###  https://w3id.org/fedecom/battery#hasLifetime
:hasLifetime rdf:type owl:ObjectProperty ;
             rdfs:subPropertyOf :hasCharacteristic ;
             rdfs:domain :Battery ;
             rdfs:range :BatteryLifetime ;
             rdfs:comment "Relates a battery to its expected operational duration." ;
             rdfs:label "has lifetime" ;
             <http://www.w3.org/2003/06/sw-vocab-status/ns#term_status> "stable" .


###  https://w3id.org/fedecom/battery#hasLossRate
:hasLossRate rdf:type owl:ObjectProperty ;
             rdfs:subPropertyOf :hasCharacteristic ;
             rdfs:domain :Battery ;
             rdfs:range :LossRate ;
             rdfs:comment "Relates a battery to the rate at which it loses energy or capacity over time." ;
             rdfs:label "has loss rate" ;
             <http://www.w3.org/2003/06/sw-vocab-status/ns#term_status> "stable" .


###  https://w3id.org/fedecom/battery#hasManufacturer
:hasManufacturer rdf:type owl:ObjectProperty ;
                 rdfs:domain :Battery ;
                 rdfs:range :Manufacturer ;
                 rdfs:comment "Links a battery to the entity (company or organization) that produced it." ;
                 rdfs:label "has manufacturer" ;
                 <http://www.w3.org/2003/06/sw-vocab-status/ns#term_status> "stable" .


###  https://w3id.org/fedecom/battery#hasModel
:hasModel rdf:type owl:ObjectProperty ;
          rdfs:domain :Battery ;
          rdfs:range :Model ;
          rdfs:comment "Links a battery to its specific product designation or identifier." ;
          rdfs:label "has model" ;
          <http://www.w3.org/2003/06/sw-vocab-status/ns#term_status> "stable" .


###  https://w3id.org/fedecom/battery#hasOpenCircuitVoltage
:hasOpenCircuitVoltage rdf:type owl:ObjectProperty ;
                       rdfs:subPropertyOf :hasCharacteristic ;
                       rdfs:comment "Relates a battery to its voltage when not connected to any load or charging source." ;
                       rdfs:label "has open circuit voltage" ;
                       <http://www.w3.org/2003/06/sw-vocab-status/ns#term_status> "stable" .


###  https://w3id.org/fedecom/battery#hasOpenCircuitVoltageOverDOD
:hasOpenCircuitVoltageOverDOD rdf:type owl:ObjectProperty ;
                              rdfs:subPropertyOf :hasOpenCircuitVoltage ;
                              rdfs:domain :Battery ;
                              rdfs:range :OpenCircuitVoltageOverDOD ;
                              rdfs:comment "Relates a battery to the functional relationship between open circuit voltage and depth of discharge." ;
                              rdfs:label "has open circuit voltage over Depth of Discharge" ;
                              <http://www.w3.org/2003/06/sw-vocab-status/ns#term_status> "stable" .


###  https://w3id.org/fedecom/battery#hasOpenCircuitVoltageOverSOC
:hasOpenCircuitVoltageOverSOC rdf:type owl:ObjectProperty ;
                              rdfs:subPropertyOf :hasOpenCircuitVoltage ;
                              rdfs:domain :Battery ;
                              rdfs:range :OpenCircuitVoltageOverSOC ;
                              rdfs:comment "Relates a battery to the functional relationship between open circuit voltage and state of charge." ;
                              rdfs:label "has open circuit voltage over State of Charge" ;
                              <http://www.w3.org/2003/06/sw-vocab-status/ns#term_status> "stable" .


###  https://w3id.org/fedecom/battery#hasPowerDelivery
:hasPowerDelivery rdf:type owl:ObjectProperty ;
                  rdfs:subPropertyOf :hasCharacteristic ;
                  rdfs:domain :Battery ;
                  rdfs:range :PowerDelivery ;
                  rdfs:comment "Relates a battery to its ability to supply power to a load." ;
                  rdfs:label "has power delivery" ;
                  <http://www.w3.org/2003/06/sw-vocab-status/ns#term_status> "stable" .


###  https://w3id.org/fedecom/battery#hasSOC
:hasSOC rdf:type owl:ObjectProperty ;
        rdfs:subPropertyOf :hasCharacteristic ;
        rdfs:domain :Battery ;
        rdfs:range :SOC ;
        rdfs:comment "Relates a battery to its current level of charge." ;
        rdfs:label "has state of charge" ;
        <http://www.w3.org/2003/06/sw-vocab-status/ns#term_status> "stable" .


###  https://w3id.org/fedecom/battery#hasStorageLevel
:hasStorageLevel rdf:type owl:ObjectProperty ;
                 rdfs:subPropertyOf :hasCharacteristic ;
                 rdfs:domain :Battery ;
                 rdfs:range :StorageLevel ;
                 rdfs:comment "Relates a battery to the amount of energy stored at a given time." ;
                 rdfs:label "has storage level" ;
                 <http://www.w3.org/2003/06/sw-vocab-status/ns#term_status> "stable" .


###  https://w3id.org/fedecom/battery#hasVoltage
:hasVoltage rdf:type owl:ObjectProperty ;
            rdfs:subPropertyOf :hasCharacteristic ;
            rdfs:domain :Battery ;
            rdfs:range :Voltage ;
            rdfs:comment "Relates a battery to its operating electrical potential difference." ;
            rdfs:label "has voltage" ;
            <http://www.w3.org/2003/06/sw-vocab-status/ns#term_status> "stable" .


#################################################################
#    Data properties
#################################################################

###  http://schema.org/name
<http://schema.org/name> rdf:type owl:DatatypeProperty .


###  https://w3id.org/fedecom/battery#conversionFactor
:conversionFactor rdf:type owl:DatatypeProperty ;
                  rdfs:label "conversion factor" ;
                  <http://www.w3.org/2003/06/sw-vocab-status/ns#term_status> "testing" .


###  https://w3id.org/fedecom/battery#conversionFactor_in
:conversionFactor_in rdf:type owl:DatatypeProperty ;
                     rdfs:subPropertyOf :conversionFactor ;
                     rdfs:label "conversion factor in" ;
                     <http://www.w3.org/2003/06/sw-vocab-status/ns#term_status> "testing" .


###  https://w3id.org/fedecom/battery#conversionFactor_out
:conversionFactor_out rdf:type owl:DatatypeProperty ;
                      rdfs:subPropertyOf :conversionFactor ;
                      rdfs:label "conversion factor out" ;
                      <http://www.w3.org/2003/06/sw-vocab-status/ns#term_status> "testing" .


###  https://w3id.org/fedecom/battery#maximum
:maximum rdf:type owl:DatatypeProperty ;
         rdfs:comment "Maximum value for a given characteristic." ;
         rdfs:label "maximum" ;
         <http://www.w3.org/2003/06/sw-vocab-status/ns#term_status> "stable" .


###  https://w3id.org/fedecom/battery#maximumCycles
:maximumCycles rdf:type owl:DatatypeProperty ;
               rdfs:comment "Maximum number of cycles." ;
               rdfs:label "maximum cycles" ;
               <http://www.w3.org/2003/06/sw-vocab-status/ns#term_status> "stable" .


###  https://w3id.org/fedecom/battery#minimum
:minimum rdf:type owl:DatatypeProperty ;
         rdfs:comment "Minimum value for a given characteristic." ;
         rdfs:label "minimum" ;
         <http://www.w3.org/2003/06/sw-vocab-status/ns#term_status> "stable" .


#################################################################
#    Classes
#################################################################

###  https://w3id.org/fedecom/battery#Battery
:Battery rdf:type owl:Class ;
         rdfs:subClassOf [ rdf:type owl:Restriction ;
                           owl:onProperty :hasChargeCurrent ;
                           owl:someValuesFrom :ChargeCurrent
                         ] ,
                         [ rdf:type owl:Restriction ;
                           owl:onProperty :hasChargePower ;
                           owl:someValuesFrom :ChargePower
                         ] ,
                         [ rdf:type owl:Restriction ;
                           owl:onProperty :hasDischargeCurrent ;
                           owl:someValuesFrom :DischargeCurrent
                         ] ,
                         [ rdf:type owl:Restriction ;
                           owl:onProperty :hasDischargePower ;
                           owl:someValuesFrom :DischargePower
                         ] ,
                         [ rdf:type owl:Restriction ;
                           owl:onProperty :hasLifetime ;
                           owl:someValuesFrom :BatteryLifetime
                         ] ,
                         [ rdf:type owl:Restriction ;
                           owl:onProperty :hasLossRate ;
                           owl:someValuesFrom :LossRate
                         ] ,
                         [ rdf:type owl:Restriction ;
                           owl:onProperty :hasManufacturer ;
                           owl:someValuesFrom :Manufacturer
                         ] ,
                         [ rdf:type owl:Restriction ;
                           owl:onProperty :hasModel ;
                           owl:someValuesFrom :Model
                         ] ,
                         [ rdf:type owl:Restriction ;
                           owl:onProperty :hasOpenCircuitVoltageOverDOD ;
                           owl:someValuesFrom :OpenCircuitVoltageOverDOD
                         ] ,
                         [ rdf:type owl:Restriction ;
                           owl:onProperty :hasOpenCircuitVoltageOverSOC ;
                           owl:someValuesFrom :OpenCircuitVoltageOverSOC
                         ] ,
                         [ rdf:type owl:Restriction ;
                           owl:onProperty :hasPowerDelivery ;
                           owl:someValuesFrom :PowerDelivery
                         ] ,
                         [ rdf:type owl:Restriction ;
                           owl:onProperty :hasSOC ;
                           owl:someValuesFrom :SOC
                         ] ,
                         [ rdf:type owl:Restriction ;
                           owl:onProperty :hasStorageLevel ;
                           owl:someValuesFrom :StorageLevel
                         ] ,
                         [ rdf:type owl:Restriction ;
                           owl:onProperty :hasVoltage ;
                           owl:someValuesFrom :Voltage
                         ] ;
         rdfs:comment "A device that stores chemical energy and converts it into electrical energy through electrochemical reactions." ;
         rdfs:label "Battery" ;
         <http://www.w3.org/2003/06/sw-vocab-status/ns#term_status> "stable" .


###  https://w3id.org/fedecom/battery#BatteryChemistryType
:BatteryChemistryType rdf:type owl:Class ;
                      rdfs:comment "The specific chemical composition and technology used in a battery." ;
                      rdfs:label "Battery chemistry type" ;
                      <http://www.w3.org/2003/06/sw-vocab-status/ns#term_status> "stable" ;
                      <http://www.w3.org/2004/02/skos/core#example> "Lithium-ion, Lead-acid, Nickel-metal hydride" .


###  https://w3id.org/fedecom/battery#BatteryLifetime
:BatteryLifetime rdf:type owl:Class ;
                 rdfs:comment "The total period a battery can function effectively before its capacity drops below a usable threshold, often measured in cycles or years." ;
                 rdfs:label "Battery lifetime" ;
                 <http://www.w3.org/2003/06/sw-vocab-status/ns#term_status> "stable" .


###  https://w3id.org/fedecom/battery#Capacity
:Capacity rdf:type owl:Class ;
          rdfs:comment "The amount of electric charge a battery can store." ;
          rdfs:label "Capacity" ;
          <http://www.w3.org/2003/06/sw-vocab-status/ns#term_status> "stable" .


###  https://w3id.org/fedecom/battery#ChargeCapacity
:ChargeCapacity rdf:type owl:Class ;
                rdfs:subClassOf :Capacity ;
                rdfs:comment "The maximum amount of charge that can be stored during charging, usually equal to the battery’s rated capacity." ;
                rdfs:label "Charge capacity" ;
                <http://www.w3.org/2003/06/sw-vocab-status/ns#term_status> "stable" .


###  https://w3id.org/fedecom/battery#ChargeCurrent
:ChargeCurrent rdf:type owl:Class ;
               rdfs:subClassOf :Current ;
               rdfs:comment "The rate at which current flows into the battery during charging." ;
               rdfs:label "Charge current" ;
               <http://www.w3.org/2003/06/sw-vocab-status/ns#term_status> "stable" .


###  https://w3id.org/fedecom/battery#ChargePower
:ChargePower rdf:type owl:Class ;
             rdfs:subClassOf :Power ;
             rdfs:comment "The rate at which energy is supplied to the battery during charging." ;
             rdfs:label "Charge power" ;
             <http://www.w3.org/2003/06/sw-vocab-status/ns#term_status> "stable" .


###  https://w3id.org/fedecom/battery#Current
:Current rdf:type owl:Class ;
         rdfs:comment "The flow of electric charge through a circuit." ;
         rdfs:label "Current" ;
         <http://www.w3.org/2003/06/sw-vocab-status/ns#term_status> "stable" .


###  https://w3id.org/fedecom/battery#DischargeCurrent
:DischargeCurrent rdf:type owl:Class ;
                  rdfs:subClassOf :Current ;
                  rdfs:comment "The rate at which current flows out of the battery during discharge." ;
                  rdfs:label "Discharge current" ;
                  <http://www.w3.org/2003/06/sw-vocab-status/ns#term_status> "stable" .


###  https://w3id.org/fedecom/battery#DischargePower
:DischargePower rdf:type owl:Class ;
                rdfs:subClassOf :Power ;
                rdfs:comment "The rate at which energy is delivered from the battery during discharge." ;
                rdfs:label "Discharge power" ;
                <http://www.w3.org/2003/06/sw-vocab-status/ns#term_status> "stable" .


###  https://w3id.org/fedecom/battery#Energy
:Energy rdf:type owl:Class ;
        rdfs:comment "The total amount of work a battery can perform." ;
        rdfs:label "Energy" ;
        <http://www.w3.org/2003/06/sw-vocab-status/ns#term_status> "stable" .


###  https://w3id.org/fedecom/battery#LossRate
:LossRate rdf:type owl:Class ;
          rdfs:comment "The rate at which a battery loses stored energy over time, often due to self-discharge or inefficiencies." ;
          rdfs:label "Loss rate" ;
          <http://www.w3.org/2003/06/sw-vocab-status/ns#term_status> "stable" .


###  https://w3id.org/fedecom/battery#Manufacturer
:Manufacturer rdf:type owl:Class ;
              rdfs:comment "The company that produces the battery." ;
              rdfs:label "Manufacturer" ;
              <http://www.w3.org/2003/06/sw-vocab-status/ns#term_status> "stable" .


###  https://w3id.org/fedecom/battery#Model
:Model rdf:type owl:Class ;
       rdfs:comment "The specific product designation or name given by the manufacturer." ;
       rdfs:label "Model" ;
       <http://www.w3.org/2003/06/sw-vocab-status/ns#term_status> "stable" .


###  https://w3id.org/fedecom/battery#OpenCircuitVoltage
:OpenCircuitVoltage rdf:type owl:Class ;
                    rdfs:subClassOf :Voltage ;
                    rdfs:comment "The voltage of a battery when it is not connected to any load or circuit (no current flowing)." ;
                    rdfs:label "Open circuit voltage" ;
                    <http://www.w3.org/2003/06/sw-vocab-status/ns#term_status> "stable" .


###  https://w3id.org/fedecom/battery#OpenCircuitVoltageOverDOD
:OpenCircuitVoltageOverDOD rdf:type owl:Class ;
                           rdfs:subClassOf :OpenCircuitVoltage ;
                           rdfs:comment "The relationship between Open Circuit Voltage and the percentage of energy discharged from the battery." ;
                           rdfs:label "Open circuit voltage over Depth of Discharge" ;
                           <http://www.w3.org/2003/06/sw-vocab-status/ns#term_status> "stable" .


###  https://w3id.org/fedecom/battery#OpenCircuitVoltageOverSOC
:OpenCircuitVoltageOverSOC rdf:type owl:Class ;
                           rdfs:subClassOf :OpenCircuitVoltage ;
                           rdfs:comment "The relationship between Open Circuit Voltage and the percentage of energy remaining in the battery." ;
                           rdfs:label "Open circuit voltage over State of Charge" ;
                           <http://www.w3.org/2003/06/sw-vocab-status/ns#term_status> "stable" .


###  https://w3id.org/fedecom/battery#Power
:Power rdf:type owl:Class ;
       rdfs:comment "How quickly the battery can deliver or absorb energy during discharge or charge" ;
       rdfs:label "Power" ;
       <http://www.w3.org/2003/06/sw-vocab-status/ns#term_status> "stable" .


###  https://w3id.org/fedecom/battery#PowerDelivery
:PowerDelivery rdf:type owl:Class ;
               rdfs:comment "The ability of the battery to supply power to a load." ;
               rdfs:label "Power delivery" ;
               <http://www.w3.org/2003/06/sw-vocab-status/ns#term_status> "stable" .


###  https://w3id.org/fedecom/battery#SOC
:SOC rdf:type owl:Class ;
     rdfs:comment "The current level of charge in the battery compared to its full capacity." ;
     rdfs:label "State of charge" ;
     <http://www.w3.org/2003/06/sw-vocab-status/ns#term_status> "stable" .


###  https://w3id.org/fedecom/battery#StorageLevel
:StorageLevel rdf:type owl:Class ;
              rdfs:comment "Indicates how much energy is stored in the battery at a given time." ;
              rdfs:label "Storage level" ;
              <http://www.w3.org/2003/06/sw-vocab-status/ns#term_status> "stable" .


###  https://w3id.org/fedecom/battery#Voltage
:Voltage rdf:type owl:Class ;
         rdfs:comment "The force that drives electric current through a circuit. It varies with the battery’s state of charge and load conditions." ;
         rdfs:label "Voltage" ;
         <http://www.w3.org/2003/06/sw-vocab-status/ns#term_status> "stable" .


###  Generated by the OWL API (version 5.1.14) https://github.com/owlcs/owlapi/
